@prefix : <http://www.semanticweb.org/sabaakram/ontologies/2024/10/untitled-ontology-7/> .
@prefix owl: <http://www.w3.org/2002/07/owl#> .
@prefix rdf: <http://www.w3.org/1999/02/22-rdf-syntax-ns#> .
@prefix xml: <http://www.w3.org/XML/1998/namespace> .
@prefix xsd: <http://www.w3.org/2001/XMLSchema#> .
@prefix rdfs: <http://www.w3.org/2000/01/rdf-schema#> .
@base <http://www.semanticweb.org/sabaakram/ontologies/2024/10/untitled-ontology-7/> .

<http://www.semanticweb.org/yourname/ontologies/movies'> rdf:type owl:Ontology .

#################################################################
#    Annotation properties
#################################################################

###  http://www.w3.org/2000/01/rdf-schema#comment
rdfs:comment rdfs:comment "This class represents films, including all metadata related to them." .


###  http://www.w3.org/2000/01/rdf-schema#label
rdfs:label rdfs:label "Movie" .


#################################################################
#    Object Properties
#################################################################

###  http://www.semanticweb.org/yourname/ontologies/movies'#belongsToGenre
:belongsToGenre rdf:type owl:ObjectProperty ;
                rdfs:domain :Movie ;
                rdfs:range :Genre ;
                rdfs:comment "This property indicates the genre category to which a particular entity, such as a movie or book, belongs." ;
                rdfs:label "Belongs to Genre" .


###  http://www.semanticweb.org/yourname/ontologies/movies'#collaboratedWith
:collaboratedWith rdf:type owl:ObjectProperty ;
                  rdfs:domain :Actor ;
                  rdfs:range :Actor ;
                  rdfs:comment "This property is used to represent a collaboration between two or more entities, such as artists or organizations, on a particular project or work." ;
                  rdfs:label "Collaborated With" .


###  http://www.semanticweb.org/yourname/ontologies/movies'#directedBy
:directedBy rdf:type owl:ObjectProperty ;
            rdfs:domain :Movie ;
            rdfs:range :Director ;
            rdfs:comment "This property specifies the director responsible for the creative direction of a film, play, or similar work." ;
            rdfs:label "Directed By" .


###  http://www.semanticweb.org/yourname/ontologies/movies'#fromCountry
:fromCountry rdf:type owl:ObjectProperty ;
             rdfs:domain :Actor ,
                         :Director ;
             rdfs:range :Country ;
             rdfs:comment "This property indicates the country of origin for an entity, such as a person, organization, or product." ;
             rdfs:label "Country" .


###  http://www.semanticweb.org/yourname/ontologies/movies'#hasActor
:hasActor rdf:type owl:ObjectProperty ;
          rdfs:domain :Movie ;
          rdfs:range :Actor ;
          rdfs:comment "This property identifies the actor or actors who perform in a film, television show, or theatrical production." ;
          rdfs:label "Has Actor" .


###  http://www.semanticweb.org/yourname/ontologies/movies'#hasDirector
:hasDirector rdf:type owl:ObjectProperty ;
             rdfs:domain :Director ;
             rdfs:range :Movie ;
             rdfs:comment "This property denotes the director associated with a particular film, show, or other creative work." ;
             rdfs:label "Has Director" .


###  http://www.semanticweb.org/yourname/ontologies/movies'#hasLanguage
:hasLanguage rdf:type owl:ObjectProperty ;
             rdfs:domain :Movie ;
             rdfs:range :Language ;
             rdfs:comment "This property indicates the language or languages in which a work is available or has been produced." ;
             rdfs:label "Has Language" .


###  http://www.semanticweb.org/yourname/ontologies/movies'#hasUserAgeGroup
:hasUserAgeGroup rdf:type owl:ObjectProperty ;
                 rdfs:domain :User ;
                 rdfs:range :AgeGroup .


###  http://www.semanticweb.org/yourname/ontologies/movies'#producedBy
:producedBy rdf:type owl:ObjectProperty ;
            rdfs:domain :Movie ;
            rdfs:range :Studio ;
            rdfs:comment "This property identifies the producer or production company responsible for financing and overseeing the creation of a work." ;
            rdfs:label "Produced By" .


###  http://www.semanticweb.org/yourname/ontologies/movies'#similarTo
:similarTo rdf:type owl:ObjectProperty ;
           rdfs:domain :Movie ;
           rdfs:range :Movie ;
           rdfs:comment "This property is used to express similarity between two entities, such as products, works, or concepts, based on certain attributes or characteristics." ;
           rdfs:label "Similar To" .


###  http://www.semanticweb.org/yourname/ontologies/movies'#wonAward
:wonAward rdf:type owl:ObjectProperty ;
          rdfs:domain :Movie ;
          rdfs:range :Award ;
          rdfs:comment "This property indicates that an entity, such as a film, book, or individual, has received a specific award or recognition." ;
          rdfs:label "Won Award" .


###  http://www.w3.org/2002/07/owl#topObjectProperty
owl:topObjectProperty rdfs:domain :Movie ;
                      rdfs:range :Genre ;
                      rdfs:comment "The most general property in the ontology hierarchy, typically used as a placeholder or superclass for all object properties." ;
                      rdfs:label "Top Object Property" .


#################################################################
#    Data properties
#################################################################

###  http://www.semanticweb.org/yourname/ontologies/movies'#hasBoxOffice
:hasBoxOffice rdf:type owl:DatatypeProperty ;
              rdfs:domain :Movie ;
              rdfs:range xsd:float ;
              rdfs:comment "This property represents the box office earnings of a movie, typically measured in currency." ;
              rdfs:label "Has Box Office" .


###  http://www.semanticweb.org/yourname/ontologies/movies'#hasRating
:hasRating rdf:type owl:DatatypeProperty ,
                    owl:FunctionalProperty ;
           rdfs:domain :Movie ;
           rdfs:range xsd:float ;
           rdfs:comment "This property represents the box office earnings of a movie, typically measured in currency." ;
           rdfs:label "Has Rating" .


###  http://www.semanticweb.org/yourname/ontologies/movies'#hasReleaseYear
:hasReleaseYear rdf:type owl:DatatypeProperty ;
                rdfs:domain :Movie ;
                rdfs:range xsd:integer ;
                rdfs:comment "This property specifies the year in which a movie, book, or other work was released or published." ;
                rdfs:label "Has Release Year" .


###  http://www.semanticweb.org/yourname/ontologies/movies'#hasReviewText
:hasReviewText rdf:type owl:DatatypeProperty ;
               rdfs:domain :Review ;
               rdfs:range xsd:string ;
               rdfs:comment "This property contains the textual content of a review, providing feedback or opinions on a particular work or product." ;
               rdfs:label "Has Review Text" .


###  http://www.semanticweb.org/yourname/ontologies/movies'#hasUserAgeGroup
:hasUserAgeGroup rdf:type owl:DatatypeProperty ;
                 rdfs:domain :User ;
                 rdfs:range xsd:integer .


#################################################################
#    Classes
#################################################################

###  http://www.semanticweb.org/yourname/ontologies/movies'#Actor
:Actor rdf:type owl:Class ;
       owl:disjointWith :Director ;
       rdfs:comment "An individual who performs in movies, playing various roles." .


###  http://www.semanticweb.org/yourname/ontologies/movies'#AgeGroup
:AgeGroup rdf:type owl:Class ;
          rdfs:comment "Categorizes viewers based on age, such as children, teens, and adults, for content suitability." ;
          rdfs:label "Age Group" .


###  http://www.semanticweb.org/yourname/ontologies/movies'#Award
:Award rdf:type owl:Class ;
       rdfs:comment "Recognition given to movies or individuals for excellence in cinematic achievements." ;
       rdfs:label "Awards" .


###  http://www.semanticweb.org/yourname/ontologies/movies'#AwardWinningMovie
:AwardWinningMovie rdf:type owl:Class ;
                   owl:equivalentClass [ rdf:type owl:Restriction ;
                                         owl:onProperty :wonAward ;
                                         owl:someValuesFrom :Award
                                       ] ;
                   rdfs:subClassOf :Movie ;
                   rdfs:label "Award-Winning Movie" ,
                              "This concept represents movies that have received one or more awards, recognizing their excellence in various aspects such as acting, directing, or technical achievements." .


###  http://www.semanticweb.org/yourname/ontologies/movies'#Blockbuster
:Blockbuster rdf:type owl:Class ;
             owl:equivalentClass [ rdf:type owl:Class ;
                                   owl:unionOf ( [ rdf:type owl:Restriction ;
                                                   owl:onProperty :hasBoxOffice ;
                                                   owl:someValuesFrom [ rdf:type rdfs:Datatype ;
                                                                        owl:onDatatype xsd:float ;
                                                                        owl:withRestrictions ( [ xsd:minInclusive "5.0E8"^^xsd:float
                                                                                               ]
                                                                                             )
                                                                      ]
                                                 ]
                                                 [ rdf:type owl:Restriction ;
                                                   owl:onProperty :hasRating ;
                                                   owl:someValuesFrom [ rdf:type rdfs:Datatype ;
                                                                        owl:onDatatype xsd:float ;
                                                                        owl:withRestrictions ( [ xsd:minInclusive "8.0"^^xsd:float
                                                                                               ]
                                                                                             )
                                                                      ]
                                                 ]
                                               )
                                 ] ;
             rdfs:subClassOf :Movie ;
             rdfs:comment "This concept refers to movies that have achieved significant commercial success, often characterized by high box office earnings and widespread popularity." ;
             rdfs:label "Blockbuster" .


###  http://www.semanticweb.org/yourname/ontologies/movies'#Box_Office
:Box_Office rdf:type owl:Class ;
            rdfs:comment "Represents the total revenue generated by a movie from ticket sales." ;
            rdfs:label "Box Office" .


###  http://www.semanticweb.org/yourname/ontologies/movies'#Collaboration
:Collaboration rdf:type owl:Class ;
               rdfs:comment "Represents the working relationship between actors or directors on a movie project." ;
               rdfs:label "Collaboration" .


###  http://www.semanticweb.org/yourname/ontologies/movies'#Country
:Country rdf:type owl:Class ;
         rdfs:comment "The nation where a movie is produced or distributed." ;
         rdfs:label "Country" .


###  http://www.semanticweb.org/yourname/ontologies/movies'#Director
:Director rdf:type owl:Class ;
          rdfs:subClassOf [ rdf:type owl:Restriction ;
                            owl:onProperty :directedBy ;
                            owl:minQualifiedCardinality "1"^^xsd:nonNegativeInteger ;
                            owl:onClass :Director
                          ] ;
          rdfs:comment "A person responsible for overseeing the artistic and dramatic aspects of a movie." ;
          rdfs:label "Director" .


###  http://www.semanticweb.org/yourname/ontologies/movies'#Genre
:Genre rdf:type owl:Class ;
       rdfs:comment "A category of movies characterized by similarities in form, style, or subject matter." ;
       rdfs:label "Genre" .


###  http://www.semanticweb.org/yourname/ontologies/movies'#Language
:Language rdf:type owl:Class ;
          rdfs:comment "Indicates the primary language spoken in a movie." ;
          rdfs:label "Language" .


###  http://www.semanticweb.org/yourname/ontologies/movies'#Movie
:Movie rdf:type owl:Class ;
       rdfs:comment "Represents a cinematic production, including feature films, documentaries, and short films." ;
       rdfs:label "Movie" .


###  http://www.semanticweb.org/yourname/ontologies/movies'#Rating
:Rating rdf:type owl:Class ;
        rdfs:subClassOf [ rdf:type owl:Restriction ;
                          owl:onProperty :hasActor ;
                          owl:minQualifiedCardinality "1"^^xsd:nonNegativeInteger ;
                          owl:onClass :Actor
                        ] ;
        rdfs:comment "An evaluation score given to a movie by users or critics, often on a scale of 1 to 10." ;
        rdfs:label "Rating" .


###  http://www.semanticweb.org/yourname/ontologies/movies'#ReleaseYear
:ReleaseYear rdf:type owl:Class ;
             rdfs:comment "The year in which a movie was officially released to the public." ;
             rdfs:label "Release Year" .


###  http://www.semanticweb.org/yourname/ontologies/movies'#Review
:Review rdf:type owl:Class ;
        rdfs:comment "A written or spoken evaluation of a movie, typically including a summary and critique." ;
        rdfs:label "Review" .


###  http://www.semanticweb.org/yourname/ontologies/movies'#Studio
:Studio rdf:type owl:Class ;
        rdfs:comment "A company or organization involved in the production and distribution of movies." ;
        rdfs:label "Studio" .


###  http://www.semanticweb.org/yourname/ontologies/movies'#User
:User rdf:type owl:Class ;
      rdfs:comment "An individual who interacts with the movie database, providing ratings or reviews." ;
      rdfs:label "User" .


#################################################################
#    Individuals
#################################################################

###  http://www.semanticweb.org/yourname/ontologies/movies'#Action
:Action rdf:type owl:NamedIndividual ,
                 :Genre .


###  http://www.semanticweb.org/yourname/ontologies/movies'#Adult
:Adult rdf:type owl:NamedIndividual ,
                :AgeGroup ;
       rdfs:comment "Refers to an age group typically 18 and over, used for content rating and demographic analysis." .


###  http://www.semanticweb.org/yourname/ontologies/movies'#China
:China rdf:type owl:NamedIndividual .


###  http://www.semanticweb.org/yourname/ontologies/movies'#ChristopherNolan
:ChristopherNolan rdf:type owl:NamedIndividual .


###  http://www.semanticweb.org/yourname/ontologies/movies'#Comedy
:Comedy rdf:type owl:NamedIndividual .


###  http://www.semanticweb.org/yourname/ontologies/movies'#Disney
:Disney rdf:type owl:NamedIndividual .


###  http://www.semanticweb.org/yourname/ontologies/movies'#Drama
:Drama rdf:type owl:NamedIndividual .


###  http://www.semanticweb.org/yourname/ontologies/movies'#English
:English rdf:type owl:NamedIndividual .


###  http://www.semanticweb.org/yourname/ontologies/movies'#France
:France rdf:type owl:NamedIndividual .


###  http://www.semanticweb.org/yourname/ontologies/movies'#French
:French rdf:type owl:NamedIndividual .


###  http://www.semanticweb.org/yourname/ontologies/movies'#Hindi
:Hindi rdf:type owl:NamedIndividual .


###  http://www.semanticweb.org/yourname/ontologies/movies'#Inception
:Inception rdf:type owl:NamedIndividual ,
                    :Movie ;
           :belongsToGenre :Action ;
           :hasRating "8.8"^^xsd:float ;
           :hasUserAgeGroup 3 ,
                            1 ,
                            2 .


###  http://www.semanticweb.org/yourname/ontologies/movies'#India
:India rdf:type owl:NamedIndividual .


###  http://www.semanticweb.org/yourname/ontologies/movies'#KathrynBigelow
:KathrynBigelow rdf:type owl:NamedIndividual .


###  http://www.semanticweb.org/yourname/ontologies/movies'#Mandarin
:Mandarin rdf:type owl:NamedIndividual .


###  http://www.semanticweb.org/yourname/ontologies/movies'#MartinScorsese
:MartinScorsese rdf:type owl:NamedIndividual .


###  http://www.semanticweb.org/yourname/ontologies/movies'#Paramount
:Paramount rdf:type owl:NamedIndividual .


###  http://www.semanticweb.org/yourname/ontologies/movies'#PulpFiction
:PulpFiction rdf:type owl:NamedIndividual .


###  http://www.semanticweb.org/yourname/ontologies/movies'#QuentinTarantino
:QuentinTarantino rdf:type owl:NamedIndividual .


###  http://www.semanticweb.org/yourname/ontologies/movies'#SciFi
:SciFi rdf:type owl:NamedIndividual .


###  http://www.semanticweb.org/yourname/ontologies/movies'#Senior
:Senior rdf:type owl:NamedIndividual ,
                 :AgeGroup ;
        rdfs:comment "Refers to an age group typically over 65, used for demographic analysis." .


###  http://www.semanticweb.org/yourname/ontologies/movies'#Spanish
:Spanish rdf:type owl:NamedIndividual .


###  http://www.semanticweb.org/yourname/ontologies/movies'#StevenSpielberg
:StevenSpielberg rdf:type owl:NamedIndividual .


###  http://www.semanticweb.org/yourname/ontologies/movies'#Teen
:Teen rdf:type owl:NamedIndividual ,
               :AgeGroup ;
      rdfs:comment "Refers to an age group typically between 13 and 19 years old, used for content rating." .


###  http://www.semanticweb.org/yourname/ontologies/movies'#TheDarkKnight
:TheDarkKnight rdf:type owl:NamedIndividual .


###  http://www.semanticweb.org/yourname/ontologies/movies'#TheGodfather
:TheGodfather rdf:type owl:NamedIndividual .


###  http://www.semanticweb.org/yourname/ontologies/movies'#Thriller
:Thriller rdf:type owl:NamedIndividual .


###  http://www.semanticweb.org/yourname/ontologies/movies'#Titanic
:Titanic rdf:type owl:NamedIndividual .


###  http://www.semanticweb.org/yourname/ontologies/movies'#UK
:UK rdf:type owl:NamedIndividual .


###  http://www.semanticweb.org/yourname/ontologies/movies'#USA
:USA rdf:type owl:NamedIndividual .


###  http://www.semanticweb.org/yourname/ontologies/movies'#UniversalPictures
:UniversalPictures rdf:type owl:NamedIndividual .


###  http://www.semanticweb.org/yourname/ontologies/movies'#WarnerBros
:WarnerBros rdf:type owl:NamedIndividual .


###  http://www.semanticweb.org/yourname/ontologies/movies'#20thCenturyFox
<http://www.semanticweb.org/yourname/ontologies/movies'#20thCenturyFox> rdf:type owl:NamedIndividual .


#################################################################
#    Annotations
#################################################################

:hasUserAgeGroup rdfs:comment "This property denotes the age group category applicable to a user or audience, often used for demographic analysis or content suitability." ;
                 rdfs:label "User Age Group" .


owl:topDataProperty rdfs:comment "The most general data property in the ontology hierarchy, typically used as a placeholder or superclass for all data properties." ;
                    rdfs:label "Top Data Property" .


###  Generated by the OWL API (version 4.5.29.2024-05-13T12:11:03Z) https://github.com/owlcs/owlapi
